fix: `letDecl`
use `simpleBinderWithoutType` at `declSig` and `optDeclSig`

tests/lean/run/newfrontend1.lean
@@ -371,3 +371,16 @@ def f1 (x : Nat) : Nat :=
   loop x
 
 #eval f1 5
+
+def f2 (x : Nat) : String :=
+  let bad x : String := toString x
+  bad x
+
+def f3 x y :=
+  x + y + 1
+
+theorem f3eq x y : f3 x y = x + y + 1 :=
+  rfl
+
+def f4 x y : String :=
+  if x > y + 1 then "hello" else "world"
