src/Lean/Parser/Term.lean
@@ -149,8 +149,10 @@ def optExprPrecedence := optional («try» ":" >> termParser maxPrec)
 -- NOTE: syntax quotations are defined in Init.Lean.Parser.Command
 @[builtinTermParser] def «match_syntax» := parser!:leadPrec "match_syntax" >> termParser >> " with " >> matchAlts
 
+def simpleBinderWithoutType := node `Lean.Parser.Term.simpleBinder (many1 binderIdent >> pushNone)
+
 /- Remark: we use `checkWsBefore` to ensure `let x[i] := e; b` is not parsed as `let x [i] := e; b` where `[i]` is an `instBinder`. -/
-def letIdLhs    : Parser := ident >> checkWsBefore "expected space before binders" >> many (ppSpace >> (simpleBinder <|> bracketedBinder)) >> optType
+def letIdLhs    : Parser := ident >> checkWsBefore "expected space before binders" >> many (ppSpace >> (simpleBinderWithoutType <|> bracketedBinder)) >> optType
 def letIdDecl   := node `Lean.Parser.Term.letIdDecl   $ «try» (letIdLhs >> " := ") >> termParser
 def letPatDecl  := node `Lean.Parser.Term.letPatDecl  $ «try» (termParser >> pushNone >> optType >> " := ") >> termParser
 def letEqnsDecl := node `Lean.Parser.Term.letEqnsDecl $ letIdLhs >> matchAlts false
